%!TEX TS-program = xelatex  
%!TEX encoding = UTF-8 Unicode  
\documentclass[12pt,a4paper]{paper}
\usepackage{float}
\usepackage{indentfirst}
\usepackage{geometry} 
\usepackage{enumitem} 
\usepackage{amsmath}  
\usepackage{braket}    
\usepackage{fontspec,xltxtra,xunicode} 


\usepackage[]{xeCJK}
\setCJKmainfont[ItalicFont=STHeitiSC-Light]{STSong}
\setCJKsansfont[BoldFont=STHeiti]{STXihei}
\setCJKmonofont{STFangsong}

%\defaultfontfeatures{Mapping=tex-text}  
%\setromanfont{SimSun} %设置中文字体  
\XeTeXlinebreaklocale “zh”  
\XeTeXlinebreakskip = 0pt plus 1pt minus 0.1pt %文章内中文自动换行  
      

\title{Black-Scholes Formula, a physicist's perspective}
\author{}
\date{\today}
\begin{document}
\maketitle
\section{(a)}
Rewritten Using $Brownian$ $Motion$: 
\begin{equation}
ds(t) = \phi s(t) dt + \sigma s(t) dW(t).
\end{equation}
where $W(t)$ is a standard brownian motion.\\\indent To illustrate the relation between \textbf{Gaussian Noise} and \textbf{Brownian Motion}, consider when using $R(t)$, we're actually suggesting $s(t + \epsilon) = s(t) + \phi s(t) \epsilon + \sigma R \epsilon$. In this case, $R \sim \mathcal{N}(0, \frac{1}{\epsilon})$, therefore $R \epsilon \sim \mathcal{N}(0, \epsilon)$, which can be characterized as $W(t + \epsilon) - W(t)$. As $\epsilon \rightarrow 0$, $W(t + \epsilon) - W(t) \rightarrow dW(t)$. (It's really clearer to use $brownian$ $motion$ notation.) Brownian motion has the property that $dW(t)dW(t) = dt$, $dW(t) dt = 0$.\\
\indent The original statement can be rewritten as: 
\begin{equation}
df(t, s(t)) = f_t dt + \frac{1}{2}\sigma^2s^2f_{ss}dt + \phi s f_s dt + \sigma s dW(t).
\end{equation}
\indent According to $Taylor$ $expansion$ $formula$, we can write
\begin{equation} 
df = f_t dt + f_s ds + \frac{1}{2}\{f_{tt} dt^2 + (f_{ts} + f_{st})dt ds(t) + f_{ss} ds(t)ds(t) \} + o(dt^2)
\end{equation} 

\begin{equation}
\Longrightarrow df = f_t dt + f_s ds + \frac{1}{2} f_{ss} ds(t)ds(t)
\end{equation}

\indent Considering $ds(t) = \phi s(t) dt + \sigma s(t) dW(t)$, $dW(t)dW(t) = dt$, $dW(t) dt = 0$, we have 
\begin{equation}
df = f_t dt + \frac{1}{2}\sigma^2s^2f_{ss}dt + \phi s f_s dt + \sigma s dW(t)
\end{equation}
\indent Using the relationship between W(t) and R(t), we can change dW(t) and derive:
\begin{equation}
\frac{df}{dt}=\frac{\partial f}{\partial t}+\frac{1}{2}\sigma ^{2}s^{2}\frac{\partial^2 f}{\partial s^2}+\frac{\partial f}{\partial s}(\phi s+\sigma sR).
\end{equation}

\section{(b)}
\indent We've already known that $c = c(t, s(t))$. Consider a portfolio $\Pi=c-\frac{\partial c}{\partial s}s$.\\
\indent To calculate the derivative of $\Pi$ we can write down the differential of $\Pi$:
\begin{equation}
d\Pi = c_t dt + c_s ds + \frac{1}{2}c_{ss} ds ds - c_s ds.
\end{equation}
\indent Because we've got $dS^2={\sigma}^{2} s^{2}dt$, we can derive:
\begin{equation}
\frac{d\Pi}{dt}= c_t + \frac{1}{2} c_{ss} \sigma^2 s^2.
\end{equation}

\section{(c)}
\indent r means the short-term risk-free interest rate. The following equation must be true:
\begin{equation}
\frac{d\Pi}{dt}=r\Pi.
\end{equation}
\indent Otherwise arbitrage will exist, which contradicts our assumption. Therefore we can write $d\Pi = r(c - c_s s)dt$. It's equivalent to the previous result $c_t dt + \frac{1}{2} c_{ss} \sigma^2 s^2 dt$.\\
\indent At last we have the \textbf{Black-Scholes formula}:
\begin{equation}
c_t + \frac{1}{2}\sigma^2 s^2 c_{ss} + rsc_s - rc = 0.
\end{equation}
\indent Why the equation does not contain $\phi$ ? \\
\indent Intuitively, it means that the expected return of an stock has nothing to do with the derivatives pricing. In other words, if there are two stocks at the same price today, which are expected to have different rate of returns in the future, will have the same the price for their derivatives, whether it be options or something else. It might seem weird at first sight because a call option should have a higher price if the the underlying stock is expected to rise up. But actually it is not. Derivatives pricing is relative pricing instead of absolute pricing. If the return is high, it might have a higher volatility. And the price of the stock today reflects every piece of information at present. So when pricing a Derivative, we just consider the price $S$, and do not include the expected return, $\phi$. It's just derived from the underlying assets.

\section*{Another Way of Obtaining B-S Formula}
According to non-arbitrage postulate, if at time $0$, $c(0, S(0)) = c_0$, then we should should be able to construct a portfolio $X(t)$(with $X(0) = c_0$) to replicate exactly this option. We should use the underlying stock $S(t)$ and the money market with interest rate $r$. Suppose we hold $\Delta(t)$ share of stock at time $t$, then it follows:
\begin{equation}
dX(t) = \Delta(t)dS(t) + r(X(t) - \Delta(t)S(t))dt = D_tdt + D_w dW(t)
\end{equation}
where $D_t = \Delta(t)S(t)(\phi - r) + r X(t)$, $D_w = \Delta(t)S(t)\sigma$.\\
\indent At the same time,
\begin{equation}
dc(t, S(t)) = c_t dt + c_s dS(t) + \frac{1}{2} c_{ss} dS(t)dS(t) = D_t' dt + D_w'dW(t)
\end{equation}
where $D_t' = c_t + c_s \phi S(t) + \frac{1}{2}\sigma^2 S(t)^2c_{ss}$, $D_w' = c_s \sigma S(t)$. \\
\indent Therefore, it should follows that $D_t = D_t', D_w = D_w'$. The second relation yields instantly that $\Delta(t) = c_s$, while the first would amount to the Black-Scholes formula:
\begin{equation}
c_t + \frac{1}{2}\sigma^2 s^2 c_{ss} + rsc_s - rc = 0
\end{equation}

\section{(d)}
Change variable $s = e^x$, we have:
\begin{equation}
c_x = e^{-x}c_s.
\end{equation}
\begin{equation}
c_t = rc - rsc_s - \frac{1}{2}\sigma^2 s^2 c_{ss} = (r - (r - \frac{1}{2}\sigma^2)\frac{\partial}{\partial x} - \frac{1}{2}\sigma^2 \frac{\partial^2}{\partial x^2}) c.
\end{equation}
\indent Therefore we can easily prove that
\begin{equation} 
H_{BS} = (1 - \frac{\partial}{\partial x})(r + \frac{1}{2} \sigma^2 \frac{\partial}{\partial x})=-\frac{\sigma ^2}{2}\frac{\partial^2 }{\partial x^2}+(\frac{\sigma ^2}{2}-r)\frac{\partial }{\partial x}+r. 
\end{equation}
which is the Hamiltonian for Black-Scholes model.

\section{(e)}
\begin{equation}
p_{BS}(x, \tau; x') = \braket{x|e^{-\tau H}|x'} = \int_{\infty}^{\infty} \frac{dp}{2\pi}\braket{x|e^{-\tau H}|p}\braket{p|x'}
\end{equation}
Taking $p = i \frac{\partial}{\partial x}$, using $\braket{x|p} = e^{ipx}$:
\begin{equation}
p_{BS}(x, \tau;x') = e^{-r\tau}\int_{\infty}^{\infty}\frac{dp}{2\pi}exp\{- \frac{1}{2}\sigma^2p^2\tau + ip(x - x') + ip\tau(r - \frac{\sigma^2}{2}) \}
\end{equation}
Finally, perform the Gaussian integration:
\begin{equation}
p_{BS}(x, \tau;x') = e^{-r\tau} \frac{1}{\sqrt{2\pi \tau \sigma^2}} exp\{ - \frac{1}{2 \sigma^2 \tau}(x - x' + \tau(r - \frac{\sigma^2}{2}) )^2 \}
\end{equation}

\section{(f)}
After obtaining the pricing kernel, we can get the price of call option at time $t$ simply by integrating the final value with the kernel.
\begin{equation}
c(\tau, x) = \int_{- \infty}^{\infty} g(x') P_{BS} dx'
\end{equation}
where in this case, $g(x') = (e^{x'} - K)^{+}$. $(x)^{+}$ takes $x$ when $x > 0$ and takes $0$ when $x \leq 0$. Therefore, the integration only takes place in $x \in (lnK, \infty)$.\par
After noticing, the pricing kernel is actually $e^{-r \tau}$ mutilpying a normal distribution, we can define $d_{-}(\tau, x) = \frac{1}{\sigma\sqrt{\tau}} [\frac{x}{lnK} + (r - \frac{1}{2}\sigma^2)\tau], d_{+} = d_{-} + \sigma \sqrt{\tau}$, $N(x) = \frac{1}{\sqrt{2\pi}}\int_{-\infty}^x e^{-\frac{x^2}{2}}$. We separate the integration into two parts: $K$ and $e^x$.\par
\begin{subequations}
\begin{align}
\int_{lnK}^{\infty} K P_{BS} dx' &= e^{-r\tau}KN(d_{-}(\tau, x)) \\
\int_{lnK}^{\infty} e^x P_{BS} dx' &= e^{x}N(d_{+}(\tau, x))
\end{align}
\end{subequations}
Remember that $s = e^{x}$, we have the pricing formula for $c(t, s)$:
\begin{equation}
c(t, s) = sN(d_{+}(\tau, s)) - e^{-r\tau} K N(d_{-}(\tau, s))
\end{equation}

With this formula, we can plot the time-evolution of stock prices and call option prices.\par
The following code does the job in $R$, results shown in $fig.1 \sim 3$
\begin{verbatim}
c_time_evolution <- function(sigma, x0, r, K)
{
    tau = seq(0, 1, 0.01)[-1]
    w = rnorm(100, 0, 0.01)
    w = cumsum(w)
    # calculate s(t)
    x = (r - 0.5*sigma^2) * tau + sigma * w
    x = exp(x)
    x = x0 * x
    #fi
    plot(tau, x, type='l')
    
    d1 = log(x/K) + (1 - tau) * (r + 0.5*sigma^2)
    d1 = d1/(sqrt(1 - tau) * sigma)
    d2 = d1 - sigma*sqrt(1 - tau)
    c = x * pnorm(d1) - exp(-r * (1-tau)) * K * pnorm(d2)
    plot(tau, c, 'l')
}
#fig.1
c_time_evolution(sigma = 0.5, x0 = 100, r = 0.20, K = 100)
#fig.2
c_time_evolution(sigma = 0.5, x0 = 80, r = 0.20, K = 100)
#fig.3
c_time_evolution(sigma = 0.5, x0 = 120, r = 0.20, K = 100)
\end{verbatim}

\begin{figure}[H]
\caption{Time-evolution of call option price}
\includegraphics[scale = 0.6]{figure1.png}
\end{figure}


\begin{figure}[H]
\caption{Time-evolution of call option price}
\includegraphics[scale = 0.6]{figure2.png}
\end{figure}


\begin{figure}[H]
\caption{Time-evolution of call option price}
\includegraphics[scale = 0.6]{figure3.png}
\end{figure}

As shown in these figures, call option price drops as $(T-t)$ decreases.

\section{(g)}
\indent Consider a down-and-out barrier European option. If $s\leq e^B(x\leq B)$ it will become worthless, which means $c=0$. \\
\indent For an arbitrary potential $v(x)$, we have:$\frac{\partial c}{\partial t}=Hc$, where $H$ can be written as:
\begin{equation}
H=-\frac{\sigma ^2}{2}\frac{\partial^2 }{\partial x^2}+(\frac{\sigma^2}{2} -r)\frac{\partial }{\partial x}+V(x).
\end{equation}
\indent Obviously, if we set $V(x)=\infty$ when $x\leq B$, then $c=0$ is automaticlly satisfied. However, when $x>B$, the changing of $c$ still conform to the B-S formula. comparing with $H_{BS}$, we have:
V(x)=
$\left\{\begin{matrix}
+\infty,x\leq B.\\
r,x>B.
\end{matrix}\right.$

\section{(h)}
\indent The Hamiltonian for the down and out option is given by:
\begin{equation}
H_{DO}=H_{BS}+V(x)=\frac{\sigma ^2}{2}\frac{\partial ^2}{\partial x^2}+(\frac{\sigma ^2}{2}-r)\frac{\partial}{\partial x}+V(x)
\end{equation}
V(x) is defined in $(g)$.\\
\indent Now we can construct the eigenfunctions similar to the $Black-Scholes$ case except that these must satisfy $\Psi _{E}(B)=0$.\\
\indent Define the quantities:
\begin{equation}
\beta =\frac{(\frac{\sigma ^2 }{2}+r)^2}{\sigma ^4}, p=\sqrt{\frac{2E}{\sigma ^2}-\beta},\alpha =\frac{\frac{\sigma ^2}{2}-r}{\sigma ^2}, i\lambda _{\pm}=\alpha \pm ip
\end{equation}
\indent The eigenfunctions are given by:
\begin{equation}
x>B:\langle x|\Psi_{E}\rangle =e^{i\lambda_{+}(x-B)}-e^{i\lambda_{-}(x-B)}=2ie^{\alpha (x-B)}\sin{[p(x-B)]}
\end{equation}
\begin{equation}
\langle \widetilde{\Psi_{E}}|x\rangle =e^{-i\lambda_{+}(x-B)}-e^{-i\lambda_{-}(x-B)}=-2ie^{-\alpha (x-B)}\sin{[p(x-B)]}
\end{equation}
\begin{equation}
\left \langle \widetilde{\Psi _{E}} | {\Psi_{E}}' \right \rangle=[2\pi \sigma ^2 \sqrt{2E/\sigma ^2 -\beta }] \delta (E-{E}').
\end{equation}
\begin{equation}
x \leq B: \left \langle x | \Psi _{E} \right \rangle=0=\left \langle \widetilde{\Psi _{E}} | x \right \rangle.
\end{equation}
\indent Now we can use the eigenfunctions to evaluate the pricing kernel. Again we work with the p variable:
\begin{align*}
\ p_{DO}(x,\tau;{x}')\
& =  \left \langle x | e^{-\tau H_{DO}} | {x}' \right \rangle \\
& = e^{-\frac{\tau \beta \sigma ^2}{2}+\alpha (x-{x}')}\int_{0}^{\infty }\frac{dp}{2\pi }e^{-\frac{1}{2}\tau \sigma ^2 p^2} [e^{ip(x-{x}')}+e^{-ip(x-{x}')}\\
& -e^{ip(x+{x}'-2B)}-e^{-ip(x+{x}'-2B)}].\
\end{align*}
\indent Consider that we have already derived:
\begin{equation}
p_{BS}(x,\tau;{x}')=e^{-r\tau}\frac{1}{\sqrt{2\pi \tau \sigma ^2}}e^{-\frac{1}{2\tau \sigma ^2}[x-{x}'+\tau(r-\frac{\sigma ^2}{2})]^2}.
\end{equation}
We can simplify the pricing kernel using the previous results:
\begin{equation}
p_{DO}(x,\tau;{x}')=p_{BS}(x,\tau;{x}')-(\frac{e^{x}}{e^{B}})^{2\alpha } p_{BS}(2B-x,\tau;{x}').
\end{equation}

\section{(i)}
We know that $r(t)$ satisfied Langevin equation:
\begin{equation}
\frac{dr}{dt}=a(r,t)+\sigma (r,t)R(t).
\end{equation}
\indent Here $R(t)$ is still Gaussian noise.\\
\indent Define the propagator $P(r,t;r_{0})$: if $r(t_0)=r_0$, the probability of $r(t)=r$ equals $P(r,t;r_{0})$.\\
\indent From the Langevin equation we have:
\begin {equation}
r(t+\varepsilon )=r(t)+\varepsilon [a+\sigma R(t)].
\end{equation}
Change it into the following formula:
\begin {equation}
r={r}'+\varepsilon [a({r}')+\sigma ({r}')R(t)].
\end{equation}
\indent Thus we can calculate the propagator:
\begin {align*}
\ P(r,t+\varepsilon ,r_{0})
& =P({r}',t;r_{0})|_{{r}'=r-\varepsilon [a({r}')+\sigma ({r}')R(t)]}\\
 &=\int P({r}',t;r_{0})\delta (r-{r}'-\varepsilon [a({r}')+\sigma ({r}')R(t)])d{r}'\\
 & \simeq \int P({r}',t;r_{0})d{r}'\{\delta (r-{r}') +\frac{\partial \delta (r-{r}')}{\partial {r}'}\varepsilon [a({r}')+\sigma ({r}')R(t)] \\
&+ \frac{1}{2}\frac{\partial^2 \delta (r-{r}')}{\partial {r}'^2} \varepsilon ^2 [a({r}')+\sigma ({r}')R(t)]^2 +... \}.\
\end{align*}
\indent Because $<R^2(t)>=\frac{1}{\varepsilon}$ and $<R(t)>=0$, the previous formula can be re-written like this:
\begin{align*}
\ P(r,t+\varepsilon ,r_{0})
& =P({r}',t;r_{0})+\int d{r}'P({r}',t;r_{0}) \{ \frac{\partial \delta (r-{r}')}{\partial {r}'}\varepsilon a({r}')+\frac{1}{2}\frac{\partial^2 \delta (r-{r}')}{\partial {r}'^2}\varepsilon ^2 \sigma ^2({r}')\frac{1}{\varepsilon } \} \\
& = P({r}',t;r_{0})-\varepsilon \frac{\partial }{\partial r}[a(r)P(r,t;r_0)]+\frac{\varepsilon }{2}\frac{\partial^2 }{\partial r^2}[\sigma (r)^2 P(r,t;r_0)].\
\end{align*}
\indent If a variable is o($\varepsilon$), it is automatically neglected.\\
\indent Thus, from the definition of derivative, we have:
\begin{equation}
\frac{\partial P(r,t;r_0)}{\partial t}=[\frac{1}{2}\frac{\partial^2 }{\partial r^2}\sigma ^2(r)-\frac{\partial }{\partial r}a(r)]P(r,t;r_0).
\end {equation}
\indent We've already known that:
\begin{equation}
\frac{\partial P(r,t;r_0)}{\partial t}=-H_{F}P(r,t;r_0).
\end{equation}
Therefore we can prove:
\begin{equation}
H_{F}=-\frac{1}{2}\frac{\partial^2 }{\partial r^2}\sigma ^2(r)+\frac{\partial }{\partial r}a(r)=-\frac{1}{2}\frac{\partial^2 }{\partial r^2}\sigma ^2(r)+a(r)\frac{\partial }{\partial r}+\frac{\partial a(r)}{\partial r}.
\end{equation}
\indent From a different perspective, we define $P_{B}(R,t;r)$ as the back propagator.\\
\indent Similarly we have( since the time flows backwards this time):
\begin{equation}
\frac{\partial P_{B}(R,t;r)}{\partial t}=+H_{B}P_{B}(R,t;r).
\end{equation}
\indent Finally we can calculate:
\begin{equation}
H_{B}=-\frac{1}{2}\sigma ^2(r)\frac{\partial^2 }{\partial r^2}-a(r)\frac{\partial }{\partial r}.
\end{equation}
$H_{B}=H_{F}^{\dag}$ is obvious.

\section{(j)}
In this part we'll focus on the so-called \textbf{stochastic Quantization}.\\
\indent The Langevin equation:
\begin{equation}
\frac{dr}{dt}=a(r,t)+\sigma (r.t)R(t)
\end{equation}
is satisfied at any time between $t_{0}$ and $T$. We must consider that both $r$ and $R$ are stochastic variables. Therefore when calculating $z_{B}$( can be compared to partition function in statistical mechanics), we must integrate over all possible paths
\begin{equation}
Z_{B}=\int DRDr\prod_{t=t_{0}}^T \delta [\frac{dr}{dc}-a(r,t)-\sigma (r,t)R(t)]e^-\frac{1}{2}\int_{t_{0}}^{T}R^2 (t)dt
\end{equation}
$Dr$ means integrating over all possible $r(t): \int Dr=\int_{-\infty}^{+\infty} \prod_{t=t_{0}}^T dr(t)$.\\
\indent We hope to write $Z_{B}$ int the form of $z_{B}=\int Dre^{s_{B}}$. Because of this, we calculate the integral over $R$ first:
\begin{equation}
Z_{B}=\int Drexp(-\frac{1}{2}\int_{t_{0}}^T \frac{[\frac{dr}{dt}-a(r,t)]^2}{\sigma^2 (r,t)}dt).
\end{equation}
\indent Because the $Dirac-\delta$ function makes sure we only keep $R(t)$ that satisfies the Langevin equation: $R(t)=\frac{\frac{dr}{dt}-a(r,t)}{\sigma (r,t)}$.\\
\indent It's easy to calculate $S_{B}$:
\begin{equation}
S_{B}=-\frac{1}{2}\int_{t_{0}}^T \frac{[\frac{dr}{dt}-a(r,t)]^2}{\sigma^2 (r,t)}dt.
\end{equation}
\indent From the definition of $S_{B}:S_{B}=\int_{t_{0}}^T Ldt,$ it's clear that:
\begin{equation}
L=-\frac{[\frac{dr}{dt}-a(r,t)]^2}{2\sigma^2 (r,t)}dt.
\end{equation}

\section{(k)}
The Vasicek model can be described using the following equation:
\begin{equation}
\frac{dr}{dt}=a(b-r)+\sigma R(t).
\end{equation}
\indent Note that if we set 
$\left\{\begin{matrix}
a(r,t)=a(b-r).\\
\sigma (r,t)=\sigma .
\end{matrix}\right.$ in Langevin equation( $a$,$b$,$\sigma$ are all constants), we have the Vasicek model naturally.\\
\indent Thus we get:
\begin{equation}
L_{V}=-\frac{[\frac{dr}{dt}-a(b-r)]^2}{2\sigma ^2}.
\end{equation}
\begin{equation}
S_{V}=-\frac{1}{2\sigma ^2}\int_{t_0}^{T}[\frac{dr}{dt}-a(b-r)]^2 dt.
\end{equation}
In the next section we'll use $S_{V}$ to calculate the propagator of Vasicek model.

\section{(l)}
\indent For different paths(which all have different $S_{V}$), so that ${e^{S_{V}}/Z}$ is the distribution of probability. $Z=\int Dr e^{S_{V}}.$
\indent Given by the question itself, we know that the propagator equals:
\begin{equation}
P(t_{0},T)=\frac{1}{Z}\int Dr e^{S_{V}} e^{-\int_{t_{0}}^{T} r(t)dt}.
\end{equation}
\indent If we use a new variable $S=S_{V}-\int_{t_{0}}^{T} r(t)dt$, then we have:
\begin{equation}
P(t_{0},T)=\frac{1}{Z}\int Dr e^{S}.
\end{equation}
\indent Change the variable: $u=r-b$. Thus we can write:
\begin{align*}
S=&-\frac{1}{2\sigma ^2}\int_{t_{0}}^{T}dt[\frac{du}{dt}+au]^2 -\int_{t_{0}}^{T}(u+b)dt\\
& =-\frac{1}{2\sigma ^2}\int_{t_{0}}^{T}dt[\frac{dr}{dt}+ar]^2 -\int_{t_{0}}^{T}(r+b)dt.
\end{align*}
\indent Next, we can define $v(t)=ar(t)+\frac{dr(t)}{dt}$. View this formula as a differential equation of $r(t)$:
\begin{equation}
\frac{dr}{dt}+ar=v(t).
\end{equation}
The solution can be easily derived:
\begin{equation}
r(t)=e^{-a(t-t_{0})}r_{0}+e^{-at}\int_{t_{0}}^{t}e^{a{t}'}v({t}')d{t}'.
\end{equation}
\indent Since we want to calculate the integral of r(t), we now have:
\begin{equation}
\int_{t_{0}}^{T}r(t)dt=B(t_{0},T)r_{0} + \int_{t_{0}}^{T} B(t,T)v(t)dt.
\end{equation}
where $B(t,T)=\frac{1-e^{-a(T-t)}}{a}$.\\
\indent From the definition of $v(t)$ we can tell that $v(T)$ is free to take all possible values. Therefore we can use the following path integral to calculate propagator:
\begin{align*}
P(t_{0}, T) &=e^{-b(T-t_{0})-B(t_{0},T)r_{0}} \frac{1}{Z}\int Dv e^{-\frac{1}{2\sigma ^2}\int_{t_0}^{T}dt[v(t)^2 + 2\sigma ^2 B(t,T)v(t)]}\\
& =e^{-b(T-t_{0})-B(t_{0},T)r_{0}} e^{\frac{\sigma ^2}{2}\int_{t_{0}}^{T}dt B(t,T)^2}.
\end{align*}
\indent The $v(t)$ integrations are decoupled Gaussian integrations, with the overall normalization being canceled by the factor Z.\\
\indent Finally, assume $B(\theta)=\frac{1-e^{-a\theta}}{a}$, where $\theta=T-t_{0}$, and $A(\theta)=exp[(\frac{\sigma^2}{2a^2}-b)(\theta -B(\theta))-\frac{\sigma ^2}{4a}B(\theta)^2]$.\\
\begin{equation}
A(\theta)e^{-r_{0}B(\theta)}=exp[-b\theta-r_{0}\frac{1-e^{-a\theta}}{a}+\frac{\sigma ^2}{2a^2}\theta - \frac{\sigma ^2 (1-e^{-a\theta})}{2a^3} +\frac{b}{a}(1-e^{-a\theta})-\frac{\sigma ^2}{4a^3}(1-e^{-a\theta})^2].
\end{equation}
\indent If we want to prove $P(t_{0},T)=A(\theta)e^{-r_{0}B(\theta)}$, then we must prove:

\begin{align*}
-b(T-t_{0})-B(t_{0},T)r_{0} +\frac{\sigma ^2}{2}& \int_{t_{0}}^{T}dt B(t,T)^2 =-b\theta-r_{0}\frac{1-e^{-a\theta}}{a}+\frac{\sigma ^2}{2a^2}\theta \\
& - \frac{\sigma ^2 (1-e^{-a\theta})}{2a^3} +\frac{b}{a}(1-e^{-a\theta})-\frac{\sigma ^2}{4a^3}(1-e^{-a\theta})^2.
\end{align*}

Change all $T-t_{0}$ to $\theta$ and all $B(t_{0},T)$ to $B(\theta)$, and calculate the integral of $B(\theta)$, we can simplify the equation:
\begin{equation}
\int_{t_{0}}^{T}\frac{(1-e^{-a\theta})^2}{a^2}dt=\frac{\theta}{a^2}-\frac{1-e^{-a\theta}}{a^3}+\frac{2b}{a\sigma ^2}(1-e^{-a\theta})-\frac{(1-e^{-a\theta})^2}{2a^3}.
\end{equation}
the left side can be written as:
\begin{equation}
\int_{t_{0}}^{T}\frac{(1-e^{-a\theta})^2}{a^2}dt=\frac{\theta}{a^2}-\frac{2}{a^3}e^{-aT}(e^{aT}-e^{at_{0}})+\frac{1}{2a^3}e^{-2aT}(e^{2aT}-e^{2at_{0}}).
\end {equation}
\indent After some comparison, the correctness is easy to prove.

\section{Conclusion}

\section{Reference}
[1]Belal E.Baaquie, Quantum Finance: Path integrals and Hamiltonians for Options and Interest Rates. Cambridge University Press (2004).
[2]Zee.A, Quantum field theory in a nutshell. Princeton university press (2010).
[3]J. C. Hull, Options, Futures and Other Derivatives. Fifth Edition, Prentice-Hall International (2003).
[4]M. Otto, ‘Using path integrals to price interest rate derivatives’, http://xxx.lanl.gov/cond-mat/9812318.
[5]O. Vasicek, ‘An Equilibrium Characterization of the Term Structure’. Journal of Financial Economics, 5: 177.
\end{document}
